%%%%%%%%%%%%%%%%%%%%%%%
\item
%%%%%%%%%%%%%%%%%%%%%%%

\begin{enumerate}[labelindent = 0pt, label = (\roman*)]
	\item $A = S_x$, $B = S_y$
	\[
		\braket{S_x}
		= \spinbra{x}{+} S_x \spinket{x}{+}
		= \braket{S_x; + | \halfhbar | S_x; +}
		= \halfhbar
	\]
	\[
		\braket{S_x^2}
		= \braket{S_x; + | S_x^2 | S_x; +}
		= \braket{S_x; + | {\left( \halfhbar \right)}^2 | S_x; +}
		= \frac{\hbar^2}{4}
	\]
	\[
		\Rightarrow \braket{{\left( \Delta S_x \right)}^2}
		= \frac{\hbar^2}{4} - {\left( \halfhbar \right)}^2
		= 0
		\; \Rightarrow
		\braket{{\left( \Delta S_x \right)}^2} \braket{{\left( \Delta S_y \right)}^2} = 0
	\]

	\vspace{10pt}

	\[
		\commutator{S_x}{S_y}
		= i\hbar S_z
		= \frac{i\hbar^2}{2} \left( \ket{+}\bra{+} - \ket{-}\bra{-} \right)
	\]
	\begin{align*}
		\Rightarrow
		\braket{\commutator{S_x}{S_y}}
		&= \braket{S_x; + | \frac{i\hbar}{2} \left( \ket{+}\bra{+} - \ket{-}\bra{-} \right) | S_x; -} \\
		&= \frac{i\hbar^2}{2}\spinbra{x}{+}\left( \sqrttwoinv (\ket{+} - \ket{-}) \right) \\
		&= 0
	\end{align*}

	\[
		\therefore
		\braket{{\left( \Delta S_x \right)}^2} \braket{{\left( \Delta S_y \right)}^2}
		\geq \frac{1}{4} {\left| \braket{\commutator{S_x}{S_y}} \right|}^2
	\]

	% =====================================

	\item $A = S_z$, $B = S_y$
	\begin{align*}
		\braket{S_z}
		&= \braket{S_x; + | \halfhbar \left( \ket{+}\bra{+} - \ket{-}\bra{-} \right) | S_x; +} \\
		&= \halfhbar \spinbra{x}{+}\left( \sqrttwoinv (\ket{+} - \ket{-}) \right) \\
		&= 0
	\end{align*}
	\[
		\braket{S_z^2}
		= \braket{S_x; + | \frac{\hbar^2}{4} \left( \ket{+}\bra{+} + \ket{-}\bra{-} \right) | S_x; +}
		= \frac{\hbar^2}{4}
	\]
	\[
		\Rightarrow \braket{{\left( \Delta S_x \right)}^2}
		= \frac{\hbar^2}{4} - 0
		= \frac{\hbar^2}{4}
	\]
	One can similarly find
	\[
		\braket{{\left( \Delta S_y \right)}^2} = \frac{\hbar^2}{4}
		\Rightarrow
		\braket{{\left( \Delta S_z \right)}^2} \braket{{\left( \Delta S_y \right)}^2}
		= \frac{\hbar^4}{16}.
	\]

	\vspace{10pt}

	\[
		\commutator{S_z}{S_y}
		= -i\hbar S_x
	\]
	\[
		\Rightarrow
		\braket{\commutator{S_z}{S_y}}
		= \braket{S_x; + | \left( -i\hbar S_x \right) | S_x; -} \\
		= -\frac{i\hbar^2}{2}
	\]
	\[
		\Rightarrow
		\frac{1}{4} {\left| \braket{\commutator{S_x}{S_y}} \right|}^2
		= \frac{\hbar^4}{16}
	\]

	\[
		\therefore
		\braket{{\left( \Delta S_x \right)}^2} \braket{{\left( \Delta S_y \right)}^2}
		\geq \frac{1}{4} {\left| \braket{\commutator{S_x}{S_y}} \right|}^2
	\]

\end{enumerate}