%%%%%%%%%%%%%%%%%%%%%%%
\item
%%%%%%%%%%%%%%%%%%%%%%%

We first observe that
\[
	\sigma_1 = \begin{pmatrix} 0 &  1 \\ 1 &  0\end{pmatrix},
	\sigma_2 = \begin{pmatrix} 0 & -i \\ i &  0\end{pmatrix},
	\sigma_3 = \begin{pmatrix} 1 &  0 \\ 0 & -1\end{pmatrix}
\]
\[
	\Rightarrow X = \begin{pmatrix}
		a_0 +  a_3 & a_1 - ia_2 \\
		a_1 + ia_2 & a_0 - a_3
	\end{pmatrix}
\]

\begin{enumerate}[labelindent = 0pt, label = (\alph*)]
	\item \[
		\sigma_1 X = \begin{pmatrix}
			a_1 + ia_2 & a_0 -  a_3 \\
			a_0 +  a_3 & a_1 - ia_2
		\end{pmatrix}
	\]
	\[
		\sigma_2 X = \begin{pmatrix}
			-ia_1 +  a_2 & -ia_0 + ia_3 \\
			 ia_0 + ia_3 &  ia_1 +  a_2
		\end{pmatrix}
	\]
	\[
		\sigma_3 X = \begin{pmatrix}
			 a_0 +  a_3 &  a_1 - ia_2 \\
			-a_1 - ia_2 & -a_0 +  a_3
		\end{pmatrix}
	\]
	\[
		\therefore \tr(X) = 2a_0,\; \tr(\sigma_k X) = 2a_k
	\]

	\item \[
		\begin{pmatrix}
			1 & 0 &  0 &  1 \\
			0 & 1 & -i &  0 \\
			0 & 1 &  i &  0 \\
			1 & 0 &  0 & -1
		\end{pmatrix}
		\begin{pmatrix}
			a_0 \\ a_1 \\ a_2 \\ a_3
		\end{pmatrix}
		=
		\begin{pmatrix}
			X_{11} \\ X_{12} \\ X_{21} \\ X_{22}
		\end{pmatrix}
	\]
	\[
		\Rightarrow
		\begin{pmatrix}
			a_0 \\ a_1 \\ a_2 \\ a_3
		\end{pmatrix}
		=
		\begin{pmatrix}
			\half & 0 & 0 & \half \\
			0 & \half & \half & 0 \\
			0 & \frac{i}{2} & -\frac{i}{2} & 0 \\
			\half & 0 & 0 & -\half
		\end{pmatrix}
		\begin{pmatrix}
			X_{11} \\ X_{12} \\ X_{21} \\ X_{22}
		\end{pmatrix}
	\]
	\[
		\therefore
		a_0 = \half(X_{11} + X_{22}),\;
		a_1 = \half(X_{12} + X_{21}),\;
		a_2 = \frac{i}{2}(X_{12} - X_{21}),\;
		a_3 = \half(X_{11} - X_{22})
	\]
\end{enumerate}
